Fix key wrapping function

crypto_hst/hmac/HMAC.Sha256.fst
@@ -27,8 +27,6 @@ let uint32s = Hacl.SBuffer.u32s
 let bytes = Hacl.SBuffer.u8s
 
 
-#set-options "--lax"
-
 
 
 val xor_bytes: output:bytes -> in1:bytes -> in2:bytes{disjoint in1 in2 /\ disjoint in1 output /\ disjoint in2 output} -> len:u32{v len <= length output /\ v len <= length in1 /\ v len <= length in2} -> STL unit
@@ -57,6 +55,7 @@ let rec xor_bytes output in1 in2 len =
 
 (* Operators *)
 let op_At_Plus (a:u32) (b:u32) : Tot u32 = UInt32.add_mod a b
+let op_Star (a:Type0) (b:Type0) : Tot Type0 = Prims.tuple2 a b
 
 
 (* Define parameters *)
@@ -64,19 +63,19 @@ let hash = Hash.Sha256.sha256
 let hl = 32ul
 let bl = 64ul
 
+#set-options "--lax"
 
 (* Define a function to wrap the key length after bl bits *)
-// BB.TODO: Uncomment the specification
-//val wrap_key : (key    :bytes) ->
-//               (keylen :u32 { length key = v keylen })
-//               -> St (okey:bytes * okeylen:u32)
-let wrap_key key keylen =
+val wrap_key : (nkey:bytes{ length nkey = v hl}) -> (key:bytes {disjoint nkey key}) -> (keylen :u32 { length key = v keylen })
+               -> STL unit
+                     (requires (fun h -> live h nkey /\ live h key))
+                     (ensures  (fun h0 _ h1 -> live h1 nkey /\ live h1 key))
+
+let wrap_key okey key keylen =
   if gt keylen bl then
-    let nkey = create (uint8_to_sint8 0uy) hl in
-    hash nkey key keylen;
-    nkey,hl
+    hash okey key keylen
   else
-    key,keylen
+    blit key 0ul okey 0ul keylen
 
 
 (* Define the main function *)
@@ -94,8 +93,12 @@ let hmac_sha256 mac key keylen data datalen =
   let ipad = create (uint8_to_sint8 0x36uy) bl in
   let opad = create (uint8_to_sint8 0x5cuy) bl in
 
+  (* Create the wrapped key location *)
+  let okeylen = bl in
+  let okey = create (uint8_to_sint8 0uy) okeylen in
+
   (* Step 1: make sure the key has the proper length *)
-  let okey,okeylen = wrap_key key keylen in
+  wrap_key okey key keylen;
   let s1 = create (uint8_to_sint8 0uy) bl in
   blit okey 0ul s1 0ul okeylen;
 
